Meta: Repair axiom tests

coq/ZF/Meta/Decl/Axiom/Extensionality.v
@@ -3,16 +3,14 @@ Require Import Coq.Strings.String.
 
 Require Import ZF.Meta.Env.
 Require Import ZF.Meta.Syntax.
-Require Import ZF.Meta.Term.Decl.
+Require Import ZF.Meta.Proof.Decl.
 Require Import ZF.Meta.Ty.
 
 Import ListNotations.
 
 (* forall a b, (forall x, x :< a <-> x :< b) -> a = b                           *)
-Definition Extensionality : DeclT :=
-  {| paraT := []
-  ;  resT  := TyProp
-  ;  bodyT :=
+Definition Extensionality : DeclP :=
+  let concl :=
       All VarTySet
         (All VarTySet
           (Imp
@@ -20,11 +18,15 @@ Definition Extensionality : DeclT :=
               (Iff (Elem (Var 0) (Var 2))
                    (Elem (Var 0) (Var 1))))
             (Equal (Var 1) (Var 0))))
-  |}.
+  in
+    {| paraP  := []
+    ;  conclP := concl
+    ;  bodyP  := AxiomP concl
+    |}.
 
 Definition imports : Env := Env.empty.
 
-Definition exports : Env := Env.fromListT
+Definition exports : Env := Env.fromListP
   [ ("Extensionality"%string, Extensionality)
   ].
 
