coq/ZF/Meta/Decl/Axiom/Foundation.v
@@ -3,7 +3,7 @@ Require Import Coq.Strings.String.
 
 Require Import ZF.Meta.Env.
 Require Import ZF.Meta.Syntax.
-Require Import ZF.Meta.Term.Decl.
+Require Import ZF.Meta.Proof.Decl.
 Require Import ZF.Meta.Ty.
 
 Import ListNotations.
@@ -12,10 +12,8 @@ Require Import ZF.Meta.Decl.Set.Empty.
 Require Import ZF.Meta.Decl.Set.Inter2.
 
 (* forall a, a <> empty -> exists x, x :< a /\ inter2 x a = empty               *)
-Definition Foundation : DeclT :=
-  {| paraT := []
-  ;  resT  := TyProp
-  ;  bodyT :=
+Definition Foundation : DeclP :=
+  let concl :=
       All VarTySet
         (Imp
           (NotEq (Var 0) (IdentT "empty" []))
@@ -25,14 +23,18 @@ Definition Foundation : DeclT :=
               (Equal
                 (IdentT "inter2" [Var 0; Var 1])
                 (IdentT "empty" [])))))
-  |}.
+  in
+    {| paraP  := []
+    ;  conclP := concl
+    ;  bodyP  := AxiomP concl
+    |}.
 
 Definition imports : Env := Env.unions
   [ Empty.exports
   ; Inter2.exports
   ].
 
-Definition exports : Env := Env.fromListT
+Definition exports : Env := Env.fromListP
   [ ("Foundation"%string, Foundation)
   ].
 
