coq/ZF/Meta/Decl/Axiom/NonEmptyUniverse.v
@@ -3,21 +3,24 @@ Require Import Coq.Strings.String.
 
 Require Import ZF.Meta.Env.
 Require Import ZF.Meta.Syntax.
-Require Import ZF.Meta.Term.Decl.
+Require Import ZF.Meta.Proof.Decl.
 Require Import ZF.Meta.Ty.
 
 Import ListNotations.
 
 (* exists x, True                                                               *)
-Definition NonEmptyUniverse : DeclT :=
-  {| paraT := []
-  ;  resT  := TyProp
-  ;  bodyT := Ex VarTySet Top
-  |}.
+Definition NonEmptyUniverse : DeclP :=
+  let concl :=
+    Ex VarTySet Top
+  in
+    {| paraP  := []
+    ;  conclP := concl
+    ;  bodyP  := AxiomP concl
+    |}.
 
 Definition imports : Env := Env.empty.
 
-Definition exports : Env := Env.fromListT
+Definition exports : Env := Env.fromListP
   [ ("NonEmptyUniverse"%string, NonEmptyUniverse)
   ].
 
