coq/ZF/Meta/Decl/Axiom/Pairing.v
@@ -3,16 +3,14 @@ Require Import Coq.Strings.String.
 
 Require Import ZF.Meta.Env.
 Require Import ZF.Meta.Syntax.
-Require Import ZF.Meta.Term.Decl.
+Require Import ZF.Meta.Proof.Decl.
 Require Import ZF.Meta.Ty.
 
 Import ListNotations.
 
 (* forall a b, exists c, forall x, x :< c <-> x = a \/ x = b                    *)
-Definition Pairing : DeclT :=
-  {| paraT := []
-  ;  resT  := TyProp
-  ;  bodyT :=
+Definition Pairing : DeclP :=
+  let concl :=
       All VarTySet
         (All VarTySet
           (Ex VarTySet
@@ -22,11 +20,15 @@ Definition Pairing : DeclT :=
                 (Or
                   (Equal (Var 0) (Var 3))
                   (Equal (Var 0) (Var 2)))))))
-  |}.
+  in
+    {| paraP  := []
+    ;  conclP := concl
+    ;  bodyP  := AxiomP concl
+    |}.
 
 Definition imports : Env := Env.empty.
 
-Definition exports : Env := Env.fromListT
+Definition exports : Env := Env.fromListP
   [ ("Pairing"%string, Pairing)
   ].
 
