coq/ZF/Meta/Decl/Axiom/Power.v
@@ -3,27 +3,29 @@ Require Import Coq.Strings.String.
 
 Require Import ZF.Meta.Env.
 Require Import ZF.Meta.Syntax.
-Require Import ZF.Meta.Term.Decl.
+Require Import ZF.Meta.Proof.Decl.
 Require Import ZF.Meta.Ty.
 
 Import ListNotations.
 
 (* forall a, exists b, forall x, x :< b <-> x <= a                              *)
-Definition Power : DeclT :=
-  {| paraT := []
-  ;  resT  := TyProp
-  ;  bodyT :=
+Definition Power : DeclP :=
+  let concl :=
       All VarTySet
         (Ex VarTySet
           (All VarTySet
             (Iff
               (Elem (Var 0) (Var 1))
               (Leq (Var 0) (Var 2)))))
-  |}.
+  in
+    {| paraP  := []
+    ;  conclP := concl
+    ;  bodyP  := AxiomP concl
+    |}.
 
 Definition imports : Env := Env.empty.
 
-Definition exports : Env := Env.fromListT
+Definition exports : Env := Env.fromListP
   [ ("Power"%string, Power)
   ].
 
