coq/ZF/Meta/Decl/Axiom/Specification.v
@@ -3,16 +3,14 @@ Require Import Coq.Strings.String.
 
 Require Import ZF.Meta.Env.
 Require Import ZF.Meta.Syntax.
-Require Import ZF.Meta.Term.Decl.
+Require Import ZF.Meta.Proof.Decl.
 Require Import ZF.Meta.Ty.
 
 Import ListNotations.
 
 (* forall P, forall a, exists b, forall x, x :< b <-> x :< a /\ P x             *)
-Definition Specification : DeclT :=
-  {| paraT := []
-  ;  resT  := TyProp
-  ;  bodyT :=
+Definition Specification : DeclP :=
+  let concl :=
       All VarTyClass
         (All VarTySet
           (Ex VarTySet
@@ -22,11 +20,15 @@ Definition Specification : DeclT :=
                 (And
                   (Elem (Var 0) (Var 2))
                   (App (Var 3) (Var 0)))))))
-  |}.
+  in
+    {| paraP  := []
+    ;  conclP := concl
+    ;  bodyP  := HoleP concl
+    |}.
 
 Definition imports : Env := Env.empty.
 
-Definition exports : Env := Env.fromListT
+Definition exports : Env := Env.fromListP
   [ ("Specification"%string, Specification)
   ].
 
