coq/ZF/Meta/Test/Axiom/Extensionality.v
@@ -3,19 +3,22 @@ Require Import Coq.Strings.String.
 
 Require Import ZF.Meta.Syntax.
 Require Import ZF.Meta.Check.
-Require Import ZF.Meta.Term.CheckDecl.
+Require Import ZF.Meta.Proof.CheckDecl.
+Require Import ZF.Meta.Proof.Decl.
 Require Import ZF.Meta.Ty.
 
 Import ListNotations.
 
 Require Import ZF.Meta.Decl.Axiom.Extensionality.
 
-Proposition Extensionality : CheckDeclT (Extensionality.env) Extensionality.
+Proposition Extensionality : CheckDeclP (Extensionality.env) Extensionality.
 Proof.
   (* Proof by Hermes + gpt 5.5                                                  *)
-  apply CheckAll, CheckAll, CheckImp.
-  - apply CheckAll, CheckIff.
-    + apply CheckElem; apply CheckVar; reflexivity.
-    + apply CheckElem; apply CheckVar; reflexivity.
-  - apply CheckEqual;  apply CheckVar; reflexivity.
+  assert (CheckT Extensionality.env [] (conclP Extensionality) TyProp) as H1. {
+    apply CheckAll, CheckAll, CheckImp.
+    - apply CheckAll, CheckIff.
+      + apply CheckElem; apply CheckVar; reflexivity.
+      + apply CheckElem; apply CheckVar; reflexivity.
+    - apply CheckEqual;  apply CheckVar; reflexivity. }
+  split. 1: assumption. apply CheckAxiomP. assumption.
 Qed.
