coq/ZF/Meta/Test/Axiom/Foundation.v
@@ -3,30 +3,33 @@ Require Import Coq.Strings.String.
 
 Require Import ZF.Meta.Syntax.
 Require Import ZF.Meta.Check.
-Require Import ZF.Meta.Term.CheckDecl.
+Require Import ZF.Meta.Proof.CheckDecl.
+Require Import ZF.Meta.Proof.Decl.
 Require Import ZF.Meta.Ty.
 
 Import ListNotations.
 
 Require Import ZF.Meta.Decl.Axiom.Foundation.
 
-Proposition Foundation : CheckDeclT (Foundation.env) Foundation.
+Proposition Foundation : CheckDeclP (Foundation.env) Foundation.
 Proof.
   (* Proof by Hermes + gpt 5.5                                                  *)
-  apply CheckAll, CheckImp.
-  - apply CheckNotEq.
-    + apply CheckVar. reflexivity.
-    + apply CheckIdentT with []. 1: reflexivity.
-      apply CheckTsNil.
-  - apply CheckEx, CheckAnd.
-    + apply CheckElem; apply CheckVar; reflexivity.
-    + apply CheckEqual.
-      * apply CheckIdentT with [TySet;TySet]. 1: reflexivity.
-        apply CheckTsCons.
-        -- apply CheckVar. reflexivity.
-        -- apply CheckTsCons.
-           ++ apply CheckVar. reflexivity.
-           ++ apply CheckTsNil.
-      * apply CheckIdentT with []. 1: reflexivity.
+  assert (CheckT Foundation.env [] (conclP Foundation) TyProp) as H1. {
+    apply CheckAll, CheckImp.
+    - apply CheckNotEq.
+      + apply CheckVar. reflexivity.
+      + apply CheckIdentT with []. 1: reflexivity.
         apply CheckTsNil.
+    - apply CheckEx, CheckAnd.
+      + apply CheckElem; apply CheckVar; reflexivity.
+      + apply CheckEqual.
+        * apply CheckIdentT with [TySet;TySet]. 1: reflexivity.
+          apply CheckTsCons.
+          -- apply CheckVar. reflexivity.
+          -- apply CheckTsCons.
+             ++ apply CheckVar. reflexivity.
+             ++ apply CheckTsNil.
+        * apply CheckIdentT with []. 1: reflexivity.
+          apply CheckTsNil. }
+  split. 1: assumption. apply CheckAxiomP. assumption.
 Qed.
