coq/ZF/Meta/Test/Axiom/Infinity.v
@@ -3,32 +3,35 @@ Require Import Coq.Strings.String.
 
 Require Import ZF.Meta.Syntax.
 Require Import ZF.Meta.Check.
-Require Import ZF.Meta.Term.CheckDecl.
+Require Import ZF.Meta.Proof.CheckDecl.
+Require Import ZF.Meta.Proof.Decl.
 Require Import ZF.Meta.Ty.
 
 Import ListNotations.
 
 Require Import ZF.Meta.Decl.Axiom.Infinity.
 
-Proposition Infinity : CheckDeclT (Infinity.env) Infinity.
+Proposition Infinity : CheckDeclP (Infinity.env) Infinity.
 Proof.
   (* Proof by Hermes + gpt 5.5                                                  *)
-  apply CheckEx, CheckAnd.
-  - apply CheckElem.
-    + apply CheckIdentT with []. 1: reflexivity.
-      apply CheckTsNil.
-    + apply CheckVar. reflexivity.
-  - apply CheckAll, CheckImp.
-    + apply CheckElem; apply CheckVar; reflexivity.
-    + apply CheckElem.
-      * apply CheckIdentT with [TySet;TySet]. 1: reflexivity.
-        apply CheckTsCons.
-        -- apply CheckVar. reflexivity.
-        -- apply CheckTsCons.
-           ++ apply CheckIdentT with [TySet]. 1: reflexivity.
-              apply CheckTsCons.
-              ** apply CheckVar. reflexivity.
-              ** apply CheckTsNil.
-           ++ apply CheckTsNil.
-      * apply CheckVar. reflexivity.
+  assert (CheckT Infinity.env [] (conclP Infinity) TyProp) as H1. {
+    apply CheckEx, CheckAnd.
+    - apply CheckElem.
+      + apply CheckIdentT with []. 1: reflexivity.
+        apply CheckTsNil.
+      + apply CheckVar. reflexivity.
+    - apply CheckAll, CheckImp.
+      + apply CheckElem; apply CheckVar; reflexivity.
+      + apply CheckElem.
+        * apply CheckIdentT with [TySet;TySet]. 1: reflexivity.
+          apply CheckTsCons.
+          -- apply CheckVar. reflexivity.
+          -- apply CheckTsCons.
+             ++ apply CheckIdentT with [TySet]. 1: reflexivity.
+                apply CheckTsCons.
+                ** apply CheckVar. reflexivity.
+                ** apply CheckTsNil.
+             ++ apply CheckTsNil.
+        * apply CheckVar. reflexivity. }
+  split. 1: assumption. apply CheckAxiomP. assumption.
 Qed.
