coq/ZF/Meta/Test/Axiom/NonEmptyUniverse.v
@@ -3,7 +3,8 @@ Require Import Coq.Strings.String.
 
 Require Import ZF.Meta.Syntax.
 Require Import ZF.Meta.Check.
-Require Import ZF.Meta.Term.CheckDecl.
+Require Import ZF.Meta.Proof.CheckDecl.
+Require Import ZF.Meta.Proof.Decl.
 Require Import ZF.Meta.Ty.
 
 Import ListNotations.
@@ -11,8 +12,10 @@ Import ListNotations.
 Require Import ZF.Meta.Decl.Axiom.NonEmptyUniverse.
 
 Proposition NonEmptyUniverse :
-  CheckDeclT (NonEmptyUniverse.env) NonEmptyUniverse.
+  CheckDeclP (NonEmptyUniverse.env) NonEmptyUniverse.
 Proof.
   (* Proof by Hermes + gpt 5.5                                                  *)
-  apply CheckEx, CheckTop.
+  assert (CheckT NonEmptyUniverse.env []
+    (conclP NonEmptyUniverse) TyProp) as H1. { apply CheckEx, CheckTop. }
+  split. 1: assumption. apply CheckAxiomP. assumption.
 Qed.
