coq/ZF/Meta/Test/Axiom/Power.v
@@ -3,17 +3,20 @@ Require Import Coq.Strings.String.
 
 Require Import ZF.Meta.Syntax.
 Require Import ZF.Meta.Check.
-Require Import ZF.Meta.Term.CheckDecl.
+Require Import ZF.Meta.Proof.CheckDecl.
+Require Import ZF.Meta.Proof.Decl.
 Require Import ZF.Meta.Ty.
 
 Import ListNotations.
 
 Require Import ZF.Meta.Decl.Axiom.Power.
 
-Proposition Power : CheckDeclT (Power.env) Power.
+Proposition Power : CheckDeclP (Power.env) Power.
 Proof.
   (* Proof by Hermes + gpt 5.5                                                  *)
-  apply CheckAll, CheckEx, CheckAll, CheckIff.
-  - apply CheckElem; apply CheckVar; reflexivity.
-  - apply CheckLeq; apply CheckVar; reflexivity.
+  assert (CheckT Power.env [] (conclP Power) TyProp) as H1. {
+    apply CheckAll, CheckEx, CheckAll, CheckIff.
+    - apply CheckElem; apply CheckVar; reflexivity.
+    - apply CheckLeq; apply CheckVar; reflexivity. }
+  split. 1: assumption. apply CheckAxiomP. assumption.
 Qed.
