coq/ZF/Meta/Test/Axiom/Replacement.v
@@ -3,31 +3,34 @@ Require Import Coq.Strings.String.
 
 Require Import ZF.Meta.Syntax.
 Require Import ZF.Meta.Check.
-Require Import ZF.Meta.Term.CheckDecl.
+Require Import ZF.Meta.Proof.CheckDecl.
+Require Import ZF.Meta.Proof.Decl.
 Require Import ZF.Meta.Ty.
 
 Import ListNotations.
 
 Require Import ZF.Meta.Decl.Axiom.Replacement.
 
-Proposition Replacement : CheckDeclT (Replacement.env) Replacement.
+Proposition Replacement : CheckDeclP (Replacement.env) Replacement.
 Proof.
   (* Proof by Hermes + gpt 5.5                                                  *)
-  apply CheckAll, CheckImp.
-  - apply CheckIdentT with [TyClass]. 1: reflexivity.
-    apply CheckTsCons.
-    + apply CheckVar. reflexivity.
-    + apply CheckTsNil.
-  - apply CheckAll, CheckEx, CheckAll, CheckIff.
-    + apply CheckElem; apply CheckVar; reflexivity.
-    + apply CheckEx, CheckAnd.
-      * apply CheckElem; apply CheckVar; reflexivity.
-      * apply CheckApp.
-        -- apply CheckVar. reflexivity.
-        -- apply CheckIdentT with [TySet;TySet]. 1: reflexivity.
-           apply CheckTsCons.
-           ++ apply CheckVar. reflexivity.
-           ++ apply CheckTsCons.
-              ** apply CheckVar. reflexivity.
-              ** apply CheckTsNil.
+  assert (CheckT Replacement.env [] (conclP Replacement) TyProp) as H1. {
+    apply CheckAll, CheckImp.
+    - apply CheckIdentT with [TyClass]. 1: reflexivity.
+      apply CheckTsCons.
+      + apply CheckVar. reflexivity.
+      + apply CheckTsNil.
+    - apply CheckAll, CheckEx, CheckAll, CheckIff.
+      + apply CheckElem; apply CheckVar; reflexivity.
+      + apply CheckEx, CheckAnd.
+        * apply CheckElem; apply CheckVar; reflexivity.
+        * apply CheckApp.
+          -- apply CheckVar. reflexivity.
+          -- apply CheckIdentT with [TySet;TySet]. 1: reflexivity.
+             apply CheckTsCons.
+             ++ apply CheckVar. reflexivity.
+             ++ apply CheckTsCons.
+                ** apply CheckVar. reflexivity.
+                ** apply CheckTsNil. }
+  split. 1: assumption. apply CheckAxiomP. assumption.
 Qed.
