coq/ZF/Meta/Test/Axiom/Specification.v
@@ -3,21 +3,24 @@ Require Import Coq.Strings.String.
 
 Require Import ZF.Meta.Syntax.
 Require Import ZF.Meta.Check.
-Require Import ZF.Meta.Term.CheckDecl.
+Require Import ZF.Meta.Proof.CheckDecl.
+Require Import ZF.Meta.Proof.Decl.
 Require Import ZF.Meta.Ty.
 
 Import ListNotations.
 
 Require Import ZF.Meta.Decl.Axiom.Specification.
 
-Proposition Specification : CheckDeclT (Specification.env) Specification.
+Proposition Specification : CheckDeclP (Specification.env) Specification.
 Proof.
   (* Proof by Hermes + gpt 5.5                                                  *)
-  apply CheckAll, CheckAll, CheckEx, CheckAll, CheckIff.
-  - apply CheckElem; apply CheckVar; reflexivity.
-  - apply CheckAnd.
-    + apply CheckElem; apply CheckVar; reflexivity.
-    + apply CheckApp.
-      * apply CheckVar. reflexivity.
-      * apply CheckVar. reflexivity.
+  assert (CheckT Specification.env [] (conclP Specification) TyProp) as H1. {
+    apply CheckAll, CheckAll, CheckEx, CheckAll, CheckIff.
+    - apply CheckElem; apply CheckVar; reflexivity.
+    - apply CheckAnd.
+      + apply CheckElem; apply CheckVar; reflexivity.
+      + apply CheckApp.
+        * apply CheckVar. reflexivity.
+        * apply CheckVar. reflexivity. }
+  split. 1: assumption. apply CheckHoleP. assumption.
 Qed.
